Begin implementing pbgr.atom

atom.lean
@@ -1,30 +1,30 @@
 import .logic
 
-class atom (α β : Type) :=
+class atom_type (α β : Type) :=
 (val : α → list β → Prop)
 (aneg : α → fm α) 
 (aneg_nqfree : ∀ (a : α), nqfree (aneg a))
-(aneg_prsv : ∀ (a : α) (xs : list β), (interp val xs (aneg a)) = (interp val xs (¬' A' a)))
+(aneg_prsv : ∀ (a : α) (xs : list β), (interp val xs (aneg a)) ↔ (interp val xs (¬' A' a)))
 (dep0 : α → Prop)
 (dec_dep0 : decidable_pred dep0)
 (decr : α → α)
-(decr_prsv : ∀ (a : α), ¬ (dep0 a) → ∀ (b : β) (bs : list β), (val (decr a) bs = val a (b::bs)))
+(decr_prsv : ∀ (a : α), ¬ (dep0 a) → ∀ (b : β) (bs : list β), (val (decr a) bs ↔ val a (b::bs)))
 (inh : β)
 (dec_eq : decidable_eq α)
 
-class atomeq (α β : Type) extends atom α β :=
+class atom_eq_type (α β : Type) extends atom_type α β :=
 (solv0 : α → Prop)
 (dec_solv0 : decidable_pred solv0)
 (dest_solv0 : ∀ a, solv0 a → nat)
 (solv0_eq : ∀ {e : α} (He : solv0 e) {b} {bs}, val e (b::bs) 
-  → list.nth_dft (atom.inh α β) (b::bs) (dest_solv0 e He) = b)
+  → list.nth_dft (atom_type.inh α β) (b::bs) (dest_solv0 e He) = b)
 (trivial : α → Prop)
 (dec_triv : decidable_pred trivial)
 (true_triv : ∀ a, trivial a → ∀ xs, val a xs)
 (subst0 : α → α → α)
 (true_subst : ∀ e, solv0 e → ∀ bs, val (subst0 e e) bs)
 (subst_prsv : ∀ {e : α} (He : solv0 e), ∀ {a : α} {bs : list β}, 
-  val (subst0 e a) bs ↔ val a ((list.nth_dft (atom.inh α β) bs (dest_solv0 e He - 1))::bs))
+  val (subst0 e a) bs ↔ val a ((list.nth_dft (atom_type.inh α β) bs (dest_solv0 e He - 1))::bs))
 (dest_pos : ∀ {a} {Ha : solv0 a}, ¬ trivial a → dest_solv0 a Ha > 0)
 
 -- Requires : j = 0 ↔ ¬(i = 0)
@@ -39,12 +39,12 @@ begin refl end
 
 variables {α β : Type}
 
-def I [atom α β] (p : fm α) (xs : list β) := interp (atom.val) xs p 
+def I [atom_type α β] (p : fm α) (xs : list β) := interp (atom_type.val) xs p 
 
-lemma exp_I_and [atom α β] (p q : fm α) (xs : list β) : 
+lemma exp_I_and [atom_type α β] (p q : fm α) (xs : list β) : 
   I (p ∧' q) xs = ((I p xs) ∧ (I q xs)) := eq.refl _
 
-lemma exp_I_and_o [atom α β] (p q : fm α) (xs : list β) : 
+lemma exp_I_and_o [atom_type α β] (p q : fm α) (xs : list β) : 
   I (and_o p q) xs = ((I p xs) ∧ (I q xs)) := 
 begin
   apply (cases_and_o' (λ p q pq, ((I pq xs) = ((I p xs) ∧ (I q xs)))) p q), 
@@ -52,10 +52,10 @@ begin
   unfold I, unfold interp 
 end
 
-lemma exp_I_or [atom α β] (p q : fm α) (xs : list β) : 
+lemma exp_I_or [atom_type α β] (p q : fm α) (xs : list β) : 
   I (p ∨' q) xs = ((I p xs) ∨ (I q xs)) := eq.refl _
 
-lemma exp_I_or_o [atom α β] (p q : fm α) (xs : list β) : 
+lemma exp_I_or_o [atom_type α β] (p q : fm α) (xs : list β) : 
   I (or_o p q) xs ↔ ((I p xs) ∨ (I q xs)) := 
 begin
   apply (cases_or_o' (λ p q pq, ((I pq xs) ↔ ((I p xs) ∨ (I q xs)))) p q), 
@@ -63,15 +63,15 @@ begin
   unfold I, unfold interp 
 end
 
-lemma exp_I_not [atom α β] (p : fm α) (xs : list β) : 
+lemma exp_I_not [atom_type α β] (p : fm α) (xs : list β) : 
   I (¬' p) xs = ¬ (I p xs) := eq.refl _
 
-lemma exp_I_ex [atom α β] (p : fm α) (xs) : @I α β _ (∃' p) xs = ∃ x, (I p (x::xs)) := 
+lemma exp_I_ex [atom_type α β] (p : fm α) (xs) : @I α β _ (∃' p) xs = ∃ x, (I p (x::xs)) := 
 by unfold I; unfold interp
 
-lemma exp_I_top [atom α β] (xs) : @I α β _ ⊤' xs = true := 
+lemma exp_I_top [atom_type α β] (xs) : @I α β _ ⊤' xs = true := 
 by unfold I; unfold interp
 
-lemma exp_I_bot [atom α β] (xs) : @I α β _ ⊥' xs = false := 
+lemma exp_I_bot [atom_type α β] (xs) : @I α β _ ⊥' xs = false := 
 by unfold I; unfold interp
 
