ldeq.lean
@@ -2,31 +2,31 @@ import .atom .ldq
 
 variables {α β : Type}
 
-open tactic atomeq
+open tactic atom_eq_type
 
-def lift_eq_qe (β : Type) [atomeq α β] (qe : list α → fm α) (as : list α) : fm α := 
-  let ntas := @list.filter _ (λ (a : α), ¬ atomeq.trivial β a) 
+def lift_eq_qe (β : Type) [atom_eq_type α β] (qe : list α → fm α) (as : list α) : fm α := 
+  let ntas := @list.filter _ (λ (a : α), ¬ atom_eq_type.trivial β a) 
     begin
       apply dec_not_pred_of_dec_pred (trivial β),  
-      apply atomeq.dec_triv
+      apply atom_eq_type.dec_triv
     end as in 
   match @list.first _ (solv0 β) 
-        begin apply atomeq.dec_solv0 end ntas with 
+        begin apply atom_eq_type.dec_solv0 end ntas with 
   | none := qe ntas 
   | some (eq,rest) := 
     list_conj  (list.map (λ (a : α), A' (subst0 β eq a)) rest)
   end
 
-lemma leq_is_dnf_qe [atomeq α β] (qe : list α → fm α) 
-  (H : ∀ (as : list α), (∀ (a : α), a ∈ as → atom.dep0 β a ∧ ¬ solv0 β a) → is_dnf_qe β qe as) : 
-  ∀ (as : list α), (∀ (a : α), a ∈ as → atom.dep0 β a) → is_dnf_qe β (lift_eq_qe β qe) as := 
+lemma leq_is_dnf_qe [atom_eq_type α β] (qe : list α → fm α) 
+  (H : ∀ (as : list α), (∀ (a : α), a ∈ as → atom_type.dep0 β a ∧ ¬ solv0 β a) → is_dnf_qe β qe as) : 
+  ∀ (as : list α), (∀ (a : α), a ∈ as → atom_type.dep0 β a) → is_dnf_qe β (lift_eq_qe β qe) as := 
 begin
   intros as Has, unfold is_dnf_qe, intros bs, 
   unfold lift_eq_qe, simp, 
   cases (@cases_first _ (solv0 β) (dec_solv0 _ β) 
     (@list.filter _ (λ (a : α), ¬trivial β a) 
       (begin apply dec_not_pred_of_dec_pred (trivial β),  
-      apply atomeq.dec_triv end) as)) with HC HC,
+      apply atom_eq_type.dec_triv end) as)) with HC HC,
   rewrite HC^.elim_left, 
   unfold lift_eq_qe, unfold is_dnf_qe at H,
   apply iff.trans, apply H, intros a Ha, 
@@ -45,27 +45,27 @@ begin
   rewrite exp_I_list_conj, rewrite map_compose, 
   
   apply iff.intro, intro HL, 
-  existsi (list.nth_dft (atom.inh α β) bs ((@atomeq.dest_solv0 α β _ eqn H2)-1)),
+  existsi (list.nth_dft (atom_type.inh α β) bs ((@atom_eq_type.dest_solv0 α β _ eqn H2)-1)),
   intros a Ha, 
   cases (dec_triv α β a) with HT HT, 
-  cases (atom.dec_eq α β a eqn) with HE HE,
-  apply (atomeq.subst_prsv H2)^.elim_left,
+  cases (atom_type.dec_eq α β a eqn) with HE HE,
+  apply (atom_eq_type.subst_prsv H2)^.elim_left,
   apply HL, apply mem_map_of_mem,
   have HM : a ∈ (eqn::as'), apply (H3 a)^.elim_left,
   apply mem_filter_of_pred_and_mem, apply HT,
   apply Ha, cases HM with HM HM, 
   apply absurd HM HE, apply HM,
   rewrite HE,  
-  apply (atomeq.subst_prsv H2)^.elim_left,
-  apply atomeq.true_subst, apply H2,
+  apply (atom_eq_type.subst_prsv H2)^.elim_left,
+  apply atom_eq_type.true_subst, apply H2,
   apply true_triv, apply HT,
   intros HR p Hp, 
   cases (ex_arg_of_mem_map Hp) with a Ha,
   cases Ha with Ha Ha', rewrite Ha', 
   clear Hp, clear Ha', clear p, 
-  apply (atomeq.subst_prsv H2)^.elim_right,
+  apply (atom_eq_type.subst_prsv H2)^.elim_right,
   cases HR with b Hb,
-  have Hbe := atomeq.solv0_eq H2 (Hb eqn _),
+  have Hbe := atom_eq_type.solv0_eq H2 (Hb eqn _),
   have H4 := (H3 a)^.elim_right _,
   rewrite (nth_dft_pred _) at Hbe,
   rewrite Hbe, apply Hb, 
@@ -78,11 +78,11 @@ begin
   apply mem_of_mem_filter H5, apply or.inl, refl
 end
 
-def lift_dnfeq_qe (β : Type) [atomeq α β] (qe : list α → fm α) := lift_dnf_qe β (@lift_eq_qe α β _ qe) 
+def lift_dnfeq_qe (β : Type) [atom_eq_type α β] (qe : list α → fm α) := lift_dnf_qe β (@lift_eq_qe α β _ qe) 
 
-lemma leq_qfree [HA : atomeq α β] (qe : list α → fm α)
-(Hqe : ∀ (as' : list α), allp (atom.dep0 β) as' → qfree (qe as'))
-(l : list α) (Hl : allp (atom.dep0 β) l) : qfree (lift_eq_qe β qe l) := 
+lemma leq_qfree [HA : atom_eq_type α β] (qe : list α → fm α)
+(Hqe : ∀ (as' : list α), allp (atom_type.dep0 β) as' → qfree (qe as'))
+(l : list α) (Hl : allp (atom_type.dep0 β) l) : qfree (lift_eq_qe β qe l) := 
 begin
   unfold lift_eq_qe, simp,
   cases (list.first (solv0 β) _) with pr,
@@ -93,8 +93,8 @@ begin
   rewrite Ha'^.elim_right, simp 
 end
 
-lemma ldeq_qfree [atomeq α β] (qe : list α → fm α) 
-  (Hqe : ∀ (as') (Has' : allp (@atom.dep0 α β _) as'), qfree (qe as')) 
+lemma ldeq_qfree [atom_eq_type α β] (qe : list α → fm α) 
+  (Hqe : ∀ (as') (Has' : allp (@atom_type.dep0 α β _) as'), qfree (qe as')) 
   (p : fm α) : qfree (lift_dnfeq_qe β qe p) := 
 begin
   unfold lift_dnfeq_qe, apply ldq_qfree, 
@@ -102,9 +102,9 @@ begin
   apply Has
 end
 
-lemma ldeq_prsv [atomeq α β] (qe : list α → fm α) 
-  (Hqe : ∀ (as) (Has : allp (@atom.dep0 α β _) as), qfree (qe as)) 
-  (Has : ∀ (as : list α), (∀ (a' : α), a' ∈ as → atom.dep0 β a' ∧ ¬ solv0 β a') → is_dnf_qe β qe as)  
+lemma ldeq_prsv [atom_eq_type α β] (qe : list α → fm α) 
+  (Hqe : ∀ (as) (Has : allp (@atom_type.dep0 α β _) as), qfree (qe as)) 
+  (Has : ∀ (as : list α), (∀ (a' : α), a' ∈ as → atom_type.dep0 β a' ∧ ¬ solv0 β a') → is_dnf_qe β qe as)  
   (p : fm α) (bs : list β) : I (lift_dnfeq_qe β qe p) bs ↔ I p bs := 
 begin
   unfold lift_dnfeq_qe, apply ldq_prsv, apply leq_qfree,
