nnf.lean
@@ -6,13 +6,13 @@ variables {α β : Type}
 Requires : qfree arg0
 Ensures : nqfree ret
 -/
-def nnf [@atom α β] : fm α → fm α 
+def nnf [@atom_type α β] : fm α → fm α 
 | (fm.true α) := ⊤'  
 | (fm.false α) := ⊥' 
 | (fm.atom a) := A' a
 | (fm.not (fm.true α)) := ⊥' 
 | (fm.not (fm.false α)) := ⊤' 
-| (fm.not (fm.atom a)) := atom.aneg β a
+| (fm.not (fm.atom a)) := atom_type.aneg β a
 | (fm.not (fm.not p)) := nnf p
 | (fm.not (fm.or p q)) := fm.and (nnf (¬' p)) (nnf (¬' q))
 | (fm.not (fm.and p q)) := fm.or (nnf (¬' p)) (nnf (¬' q))
@@ -21,27 +21,27 @@ def nnf [@atom α β] : fm α → fm α
 | (fm.and p q) := fm.and (nnf p) (nnf q)
 | (fm.ex p) := ⊥' -- Invalid input
 
-lemma nnf_exp_and [atom α β] (p q : fm α) :
+lemma nnf_exp_and [atom_type α β] (p q : fm α) :
 @nnf α β _ (fm.and p q) = fm.and (@nnf α β _ p) (@nnf α β _ q) := 
 by unfold nnf
 
-lemma nnf_exp_or [atom α β] (p q : fm α) : 
+lemma nnf_exp_or [atom_type α β] (p q : fm α) : 
 @nnf α β _ (p ∨' q) = (@nnf α β _ p ∨' @nnf α β _ q) := by unfold nnf
 
-lemma nnf_exp_not_and [H : atom α β] (p q : fm α) : 
+lemma nnf_exp_not_and [H : atom_type α β] (p q : fm α) : 
 @nnf α β _ (¬' (p ∧' q)) = (@nnf α β _ (¬' p) ∨' @nnf α β _ (¬' q)) := 
 by unfold nnf
 
-lemma nnf_exp_not_or [H : atom α β] (p q : fm α) : 
+lemma nnf_exp_not_or [H : atom_type α β] (p q : fm α) : 
 @nnf α β _ (¬' (p ∨' q)) = (@nnf α β _ (¬' p) ∧' @nnf α β _ (¬' q)) := 
 by unfold nnf
 
-lemma nqfree_not_eq_nqfree [atom α β] : ∀ (p : fm α) (Hp : qfree p), 
+lemma nqfree_not_eq_nqfree [atom_type α β] : ∀ (p : fm α) (Hp : qfree p), 
 nqfree (@nnf α β _ (¬' p)) = nqfree (@nnf α β _  p) :=
 λ p, fm.rec_on p 
   (λ _, eq.refl _) 
   (λ _, eq.refl _) 
-  (λ _ a, propext (iff.intro (λ _, trivial) (λ H, atom.aneg_nqfree _ _)))
+  (λ _ a, propext (iff.intro (λ _, trivial) (λ H, atom_type.aneg_nqfree _ _)))
   (λ q r Hq Hr Hqr,  
     begin
        unfold nnf, unfold nqfree, 
@@ -59,7 +59,7 @@ nqfree (@nnf α β _ (¬' p)) = nqfree (@nnf α β _  p) :=
       cases Hp 
     end)
 
-lemma nnf_nqfree [atom α β] : 
+lemma nnf_nqfree [atom_type α β] : 
   ∀ (p : fm α), qfree p → nqfree (@nnf α β _ p) := 
 λ p, fm.rec_on p  
 (λ _, trivial) 
@@ -78,7 +78,7 @@ lemma nnf_nqfree [atom α β] :
 (λ q, fm.rec_on q 
   (λ _ _, trivial) 
   (λ _ _, trivial) 
-  (λ _ _ _, by apply atom.aneg_nqfree) 
+  (λ _ _ _, by apply atom_type.aneg_nqfree) 
   (λ r s Hr Hs H1 H2, 
     begin
       rewrite nnf_exp_not_and,
@@ -109,13 +109,13 @@ meta def nnf_prsv_lit : tactic unit :=
 `[apply and.intro, refl, unfold nnf, 
   unfold I, unfold interp, simp]
 
-lemma nnf_prsv_core [atom α β] : ∀ (p : fm α), qfree p → 
-  (∀ (xs : list β), (I (@nnf α β _ p) xs = I p xs) ∧ (I (@nnf α β _ ¬' p) xs = I (¬' p) xs))   
+lemma nnf_prsv_core [atom_type α β] : ∀ (p : fm α), qfree p → 
+  (∀ (xs : list β), (I (@nnf α β _ p) xs ↔ I p xs) ∧ (I (@nnf α β _ ¬' p) xs ↔ I (¬' p) xs))   
 | (fm.true α)  Hp xs := by nnf_prsv_lit
 | (fm.false α) Hp xs := by nnf_prsv_lit
 | (fm.atom a)  Hp xs := 
   by {apply and.intro, refl, 
-      unfold nnf, apply atom.aneg_prsv} 
+      unfold nnf, apply atom_type.aneg_prsv} 
 | (fm.and p q) Hp xs := 
   and.intro
     (begin
@@ -129,7 +129,7 @@ lemma nnf_prsv_core [atom α β] : ∀ (p : fm α), qfree p →
       rewrite (nnf_prsv_core p _ xs)^.elim_right,
       rewrite (nnf_prsv_core q _ xs)^.elim_right,
       repeat {rewrite exp_I_not}, rewrite exp_I_and, 
-      apply propext, apply iff_not_and, 
+      apply iff_not_and, 
       apply Hp^.elim_right, apply Hp^.elim_left
      end)
 | (fm.or p q)  Hp xs := 
@@ -145,7 +145,7 @@ lemma nnf_prsv_core [atom α β] : ∀ (p : fm α), qfree p →
       rewrite (nnf_prsv_core p _ xs)^.elim_right,
       rewrite (nnf_prsv_core q _ xs)^.elim_right,
       repeat {rewrite exp_I_not}, rewrite exp_I_or, 
-      apply propext, apply iff_not_or, 
+      apply iff_not_or, 
       apply Hp^.elim_right, apply Hp^.elim_left
      end)
 | (fm.not p) Hp xs := 
@@ -154,10 +154,10 @@ lemma nnf_prsv_core [atom α β] : ∀ (p : fm α), qfree p →
     (begin 
       unfold nnf, repeat {rewrite exp_I_not}, 
       rewrite (nnf_prsv_core p Hp xs)^.elim_left, 
-      apply propext, apply iff_not_not
+      apply iff_not_not
      end)
 | (fm.ex p) Hp xs := by cases Hp
 
-lemma nnf_prsv [atom α β] (p : fm α) (Hp : qfree p) (xs : list β) : 
-I (@nnf α β _ p) xs = I p xs := (nnf_prsv_core p Hp xs)^.elim_left
+lemma nnf_prsv [atom_type α β] (p : fm α) (Hp : qfree p) (xs : list β) : 
+I (@nnf α β _ p) xs ↔ I p xs := (nnf_prsv_core p Hp xs)^.elim_left
 
