dnf.lean
@@ -1,4 +1,4 @@
-import .atom 
+import .atom
 
 variables {α β : Type}
 
@@ -13,8 +13,8 @@ def dnf : fm α → list (list α)
 | (fm.or p q) := dnf p ++ dnf q 
 | _ := []
 
-lemma dnf_prsv [atom α β] : ∀ (p : fm α) (H : nqfree p) (xs : list β), 
-  disj_list (list.map (λ (as : list α), ∀ a, a ∈ as → atom.val a xs) (dnf p)) ↔ I p xs 
+lemma dnf_prsv [atom_type α β] : ∀ (p : fm α) (H : nqfree p) (xs : list β), 
+  disj_list (list.map (λ (as : list α), ∀ a, a ∈ as → atom_type.val a xs) (dnf p)) ↔ I p xs 
 | (fm.true α) H bs := 
   by {unfold dnf, simp, unfold disj_list, 
       rewrite exp_I_top, simp}
@@ -42,7 +42,7 @@ lemma dnf_prsv [atom α β] : ∀ (p : fm α) (H : nqfree p) (xs : list β),
     simp at Hd, 
     apply and.intro, 
 
-    existsi (∀ (a : α), a ∈ (prod.fst d) → atom.val a bs),
+    existsi (∀ (a : α), a ∈ (prod.fst d) → atom_type.val a bs),
     apply and.intro, apply mem_map_of_mem,
     apply fst_mem_of_mem_product Hd^.elim_right,
     intros a Ha, rewrite Hd^.elim_left at Hrr,
@@ -50,7 +50,7 @@ lemma dnf_prsv [atom α β] : ∀ (p : fm α) (H : nqfree p) (xs : list β),
     apply mem_append_of_mem_or_mem,
     apply or.inl Ha, 
 
-    existsi (∀ (a : α), a ∈ (prod.snd d) → atom.val a bs),
+    existsi (∀ (a : α), a ∈ (prod.snd d) → atom_type.val a bs),
     apply and.intro, apply mem_map_of_mem, 
     apply snd_mem_of_mem_product Hd^.elim_right,
     intros a Ha, rewrite Hd^.elim_left at Hrr,
@@ -63,7 +63,7 @@ lemma dnf_prsv [atom α β] : ∀ (p : fm α) (H : nqfree p) (xs : list β),
     cases (H0^.elim_right) with s Hs, clear H0, 
     cases (ex_arg_of_mem_map Hr^.elim_left) with ll Hll,
     cases (ex_arg_of_mem_map Hs^.elim_left) with lr Hlr,
-    existsi (∀ (a : α), a ∈ append_pair (ll,lr) → atom.val a bs),
+    existsi (∀ (a : α), a ∈ append_pair (ll,lr) → atom_type.val a bs),
     apply and.intro, apply mem_map_of_mem, 
     apply mem_product_of_mem_of_mem,
     apply Hll^.elim_left, apply Hlr^.elim_left,
