pbgr.lean
@@ -1,0 +1,85 @@
+import .atom .auxiliary
+
+namespace pbgr 
+
+variables {α β : Type}
+
+inductive atom : Type 
+| le : int → list int → atom
+| dvd : int → int → list int → atom
+| ndvd : int → int → list int → atom
+
+def dec_eq : decidable_eq atom := 
+by tactic.mk_dec_eq_instance
+
+open atom 
+
+def divides (m n : int) : Prop := int.rem n m = 0
+
+def val : atom → list int → Prop 
+| (le i ks) xs := i ≤ dot_prod ks xs
+| (dvd d i ks) xs := divides d (i + dot_prod ks xs)
+| (ndvd d i ks) xs := ¬ (divides d (i + dot_prod ks xs))
+
+def aneg : atom → fm atom
+| (le i ks) := fm.atom (atom.le (1 - i) (list.map has_neg.neg ks))
+| (dvd d i ks)  := fm.atom (ndvd d i ks)
+| (ndvd d i ks) := fm.atom (dvd d i ks)
+
+def aneg_prsv : ∀ (a : atom) (xs : list ℤ), interp val xs (aneg a) ↔ interp val xs (¬' A' a) 
+| (le i ks)     xs := 
+  begin 
+    unfold aneg, unfold interp, 
+    unfold val, 
+    apply 
+    (calc 
+          (1 - i ≤ dot_prod (list.map has_neg.neg ks) xs) 
+        ↔ (has_neg.neg (dot_prod (list.map has_neg.neg ks) xs) ≤ has_neg.neg (1 - i)) : 
+          by {apply iff.intro, apply neg_le_neg, apply le_of_neg_le_neg}
+    ... ↔ (dot_prod ks xs ≤ has_neg.neg (1 - i)) : 
+          begin rewrite (@exp_neg_dot_prod int _ ks xs), simp, end
+    ... ↔ (dot_prod ks xs ≤ i - 1) : 
+           by rewrite neg_sub
+    ... ↔ (dot_prod ks xs < i) : 
+          begin
+            apply iff.intro,
+            apply int.lt_of_le_sub_one,
+            apply int.le_sub_one_of_lt 
+          end
+    ... ↔ ¬i ≤ dot_prod ks xs : 
+          begin
+            apply iff.intro,
+            apply not_le_of_gt,
+            apply lt_of_not_ge
+          end )
+  end
+| (dvd d i ks)  xs := by refl
+| (ndvd d i ks) xs := by apply iff_not_not
+
+def decr : atom → atom 
+| (le i ks)     := le i (list.tail ks)
+| (dvd d i ks)  := dvd d i (list.tail ks)
+| (ndvd d i ks) := ndvd d i (list.tail ks)
+
+def hd_coeff : atom → int 
+| (le i ks)     := list.head_dft 0 ks
+| (dvd d i ks)  := list.head_dft 0 ks
+| (ndvd d i ks) := list.head_dft 0 ks
+
+def dep0 (a) := hd_coeff a ≠ 0
+
+instance : atom_type atom int := 
+{ val := val,
+  aneg := aneg,
+  aneg_nqfree := 
+    begin intro a, cases a; trivial, end,
+  aneg_prsv := aneg_prsv,
+  dep0 := dep0,
+  dec_dep0 := 
+    begin intro a, apply dec_not_pred_of_dec_pred end,
+  decr := decr,
+  decr_prsv := sorry ,
+  inh := 0,
+  dec_eq := dec_eq }
+
+end pbgr
